src/proof/k8s_io/apimachinery/pkg/api/meta.v
@@ -15,7 +15,7 @@ Context {sem : go.Semantics}
 Local Set Default Proof Using "All".
 
 Lemma wp_Accessor i l o:
-  {{{ "Hinit" ∷ is_pkg_init code.k8s_io.apimachinery.pkg.api.meta.pkg_id.meta ∗
+  {{{ is_pkg_init code.k8s_io.apimachinery.pkg.api.meta.pkg_id.meta ∗
       "%Hi" ∷ ⌜ KObjectV.valid_interface i l o ⌝
   }}}
     @! code.k8s_io.apimachinery.pkg.api.meta.meta.Accessor #(interface.ok i)
@@ -32,7 +32,7 @@ Qed.
 (** The borrowed-labels rule after method promotion through a supported
     Kubernetes object interface. *)
 Lemma wp_GetLabels_deepown_kobject i l o meta dq :
-  {{{ "Hinit" ∷ is_pkg_init code.k8s_io.apimachinery.pkg.apis.meta.v1.pkg_id.v1 ∗
+  {{{ is_pkg_init code.k8s_io.apimachinery.pkg.apis.meta.v1.pkg_id.v1 ∗
       "%Hi" ∷ ⌜ KObjectV.valid_interface i l o ⌝ ∗
       "Hmeta" ∷ ObjectMetaV.deepown_l (KObjectV.objectmeta_ptr l o) meta dq
   }}}
@@ -45,12 +45,12 @@ Lemma wp_GetLabels_deepown_kobject i l o meta dq :
 Proof.
   wp_start as "H". iNamed "H".
   destruct o; simpl in Hi; destruct Hi as [-> _]; wp_method_call;
-    wp_pures; wp_apply (wp_GetLabels_deepown with "[$Hinit $Hmeta]");
+    wp_pures; wp_apply (wp_GetLabels_deepown with "[$Hmeta]");
     iIntros (labels_l) "Hlabels"; iApply "HΦ"; iFrame.
 Qed.
 
 Lemma wp_GetName_deepown_kobject i l o m dq:
-  {{{ "Hinit" ∷ is_pkg_init code.k8s_io.apimachinery.pkg.apis.meta.v1.pkg_id.v1 ∗
+  {{{ is_pkg_init code.k8s_io.apimachinery.pkg.apis.meta.v1.pkg_id.v1 ∗
       "%Hi" ∷ ⌜ KObjectV.valid_interface i l o ⌝ ∗
       "Hmeta" ∷ ObjectMetaV.deepown_l (KObjectV.objectmeta_ptr l o) m dq
   }}}
@@ -61,12 +61,12 @@ Lemma wp_GetName_deepown_kobject i l o m dq:
 Proof.
   wp_start as "H". iNamed "H".
   destruct o; simpl in Hi; destruct Hi as [-> _]; wp_method_call;
-    wp_pures; wp_apply (wp_GetName_deepown with "[$Hinit $Hmeta]");
+    wp_pures; wp_apply (wp_GetName_deepown with "[$Hmeta]");
     iIntros "Hmeta"; iApply "HΦ"; iFrame.
 Qed.
 
 Lemma wp_GetGenerateName_deepown_kobject i l o m dq:
-  {{{ "Hinit" ∷ is_pkg_init code.k8s_io.apimachinery.pkg.apis.meta.v1.pkg_id.v1 ∗
+  {{{ is_pkg_init code.k8s_io.apimachinery.pkg.apis.meta.v1.pkg_id.v1 ∗
       "%Hi" ∷ ⌜ KObjectV.valid_interface i l o ⌝ ∗
       "Hmeta" ∷ ObjectMetaV.deepown_l (KObjectV.objectmeta_ptr l o) m dq
   }}}
@@ -77,12 +77,12 @@ Lemma wp_GetGenerateName_deepown_kobject i l o m dq:
 Proof.
   wp_start as "H". iNamed "H".
   destruct o; simpl in Hi; destruct Hi as [-> _]; wp_method_call;
-    wp_pures; wp_apply (wp_GetGenerateName_deepown with "[$Hinit $Hmeta]");
+    wp_pures; wp_apply (wp_GetGenerateName_deepown with "[$Hmeta]");
     iIntros "Hmeta"; iApply "HΦ"; iFrame.
 Qed.
 
 Lemma wp_GetUID_deepown_kobject i l o m dq:
-  {{{ "Hinit" ∷ is_pkg_init code.k8s_io.apimachinery.pkg.apis.meta.v1.pkg_id.v1 ∗
+  {{{ is_pkg_init code.k8s_io.apimachinery.pkg.apis.meta.v1.pkg_id.v1 ∗
       "%Hi" ∷ ⌜ KObjectV.valid_interface i l o ⌝ ∗
       "Hmeta" ∷ ObjectMetaV.deepown_l (KObjectV.objectmeta_ptr l o) m dq
   }}}
@@ -93,12 +93,12 @@ Lemma wp_GetUID_deepown_kobject i l o m dq:
 Proof.
   wp_start as "H". iNamed "H".
   destruct o; simpl in Hi; destruct Hi as [-> _]; wp_method_call;
-    wp_pures; wp_apply (wp_GetUID_deepown with "[$Hinit $Hmeta]");
+    wp_pures; wp_apply (wp_GetUID_deepown with "[$Hmeta]");
     iIntros "Hmeta"; iApply "HΦ"; iFrame.
 Qed.
 
 Lemma wp_GetResourceVersion_deepown_kobject i l o m dq:
-  {{{ "Hinit" ∷ is_pkg_init code.k8s_io.apimachinery.pkg.apis.meta.v1.pkg_id.v1 ∗
+  {{{ is_pkg_init code.k8s_io.apimachinery.pkg.apis.meta.v1.pkg_id.v1 ∗
       "%Hi" ∷ ⌜ KObjectV.valid_interface i l o ⌝ ∗
       "Hmeta" ∷ ObjectMetaV.deepown_l (KObjectV.objectmeta_ptr l o) m dq
   }}}
@@ -109,30 +109,29 @@ Lemma wp_GetResourceVersion_deepown_kobject i l o m dq:
 Proof.
   wp_start as "H". iNamed "H".
   destruct o; simpl in Hi; destruct Hi as [-> _]; wp_method_call;
-    wp_pures; wp_apply (wp_GetResourceVersion_deepown with "[$Hinit $Hmeta]");
+    wp_pures; wp_apply (wp_GetResourceVersion_deepown with "[$Hmeta]");
     iIntros "Hmeta"; iApply "HΦ"; iFrame.
 Qed.
 
 Lemma wp_SetName_deepown_kobject i l o m name:
-  {{{ "Hinit" ∷ is_pkg_init code.k8s_io.apimachinery.pkg.apis.meta.v1.pkg_id.v1 ∗
+  {{{ is_pkg_init code.k8s_io.apimachinery.pkg.apis.meta.v1.pkg_id.v1 ∗
       "%Hi" ∷ ⌜ KObjectV.valid_interface i l o ⌝ ∗
       "Hmeta" ∷ ObjectMetaV.deepown_l (KObjectV.objectmeta_ptr l o) m 1
   }}}
     #(methods i.(interface.ty) "SetName" i.(interface.v)) #name
   {{{ RET #();
-      ObjectMetaV.deepown_l (KObjectV.objectmeta_ptr l o)
-        (m <| ObjectMetaV.Name' := name |>) 1
+      ObjectMetaV.deepown_l (KObjectV.objectmeta_ptr l o) (m <| ObjectMetaV.Name' := name |>) 1
   }}}.
 Proof.
   wp_start as "H". iNamed "H".
   destruct o; simpl in Hi; destruct Hi as [-> _]; wp_method_call;
-    wp_pures; wp_apply (wp_SetName_deepown with "[$Hinit $Hmeta]");
+    wp_pures; wp_apply (wp_SetName_deepown with "[$Hmeta]");
     iIntros "Hmeta"; iApply "HΦ"; iFrame.
 Qed.
 
 Lemma wp_SetCreationTimestamp_deepown_kobject
     i l o m creation_timestamp pure_creation_timestamp:
-  {{{ "Hinit" ∷ is_pkg_init code.k8s_io.apimachinery.pkg.apis.meta.v1.pkg_id.v1 ∗
+  {{{ is_pkg_init code.k8s_io.apimachinery.pkg.apis.meta.v1.pkg_id.v1 ∗
       "%Hi" ∷ ⌜ KObjectV.valid_interface i l o ⌝ ∗
       "Hmeta" ∷ ObjectMetaV.deepown_l (KObjectV.objectmeta_ptr l o) m 1 ∗
       "Htime" ∷ TimeV.deepown creation_timestamp pure_creation_timestamp 1
@@ -140,54 +139,51 @@ Lemma wp_SetCreationTimestamp_deepown_kobject
     #(methods i.(interface.ty) "SetCreationTimestamp" i.(interface.v))
       #creation_timestamp
   {{{ RET #();
-      ObjectMetaV.deepown_l (KObjectV.objectmeta_ptr l o)
-        (m <| ObjectMetaV.CreationTimestamp' := pure_creation_timestamp |>) 1
+      ObjectMetaV.deepown_l (KObjectV.objectmeta_ptr l o) (m <| ObjectMetaV.CreationTimestamp' := pure_creation_timestamp |>) 1
   }}}.
 Proof.
   wp_start as "H". iNamed "H".
   destruct o; simpl in Hi; destruct Hi as [-> _]; wp_method_call;
     wp_pures;
-    wp_apply (wp_SetCreationTimestamp_deepown with "[$Hinit $Hmeta $Htime]");
+    wp_apply (wp_SetCreationTimestamp_deepown with "[$Hmeta $Htime]");
     iIntros "Hmeta"; iApply "HΦ"; iFrame.
 Qed.
 
 Lemma wp_SetUID_deepown_kobject i l o m uid:
-  {{{ "Hinit" ∷ is_pkg_init code.k8s_io.apimachinery.pkg.apis.meta.v1.pkg_id.v1 ∗
+  {{{ is_pkg_init code.k8s_io.apimachinery.pkg.apis.meta.v1.pkg_id.v1 ∗
       "%Hi" ∷ ⌜ KObjectV.valid_interface i l o ⌝ ∗
       "Hmeta" ∷ ObjectMetaV.deepown_l (KObjectV.objectmeta_ptr l o) m 1
   }}}
     #(methods i.(interface.ty) "SetUID" i.(interface.v)) #uid
   {{{ RET #();
-      ObjectMetaV.deepown_l (KObjectV.objectmeta_ptr l o)
-        (m <| ObjectMetaV.UID' := uid |>) 1
+      ObjectMetaV.deepown_l (KObjectV.objectmeta_ptr l o) (m <| ObjectMetaV.UID' := uid |>) 1
   }}}.
 Proof.
   wp_start as "H". iNamed "H".
   destruct o; simpl in Hi; destruct Hi as [-> _]; wp_method_call;
-    wp_pures; wp_apply (wp_SetUID_deepown with "[$Hinit $Hmeta]");
+    wp_pures; wp_apply (wp_SetUID_deepown with "[$Hmeta]");
     iIntros "Hmeta"; iApply "HΦ"; iFrame.
 Qed.
 
 Lemma wp_SetResourceVersion_deepown_kobject i l o m resource_version:
-  {{{ "Hinit" ∷ is_pkg_init code.k8s_io.apimachinery.pkg.apis.meta.v1.pkg_id.v1 ∗
+  {{{ is_pkg_init code.k8s_io.apimachinery.pkg.apis.meta.v1.pkg_id.v1 ∗
       "%Hi" ∷ ⌜ KObjectV.valid_interface i l o ⌝ ∗
       "Hmeta" ∷ ObjectMetaV.deepown_l (KObjectV.objectmeta_ptr l o) m 1
   }}}
     #(methods i.(interface.ty) "SetResourceVersion" i.(interface.v))
       #resource_version
   {{{ RET #();
-      ObjectMetaV.deepown_l (KObjectV.objectmeta_ptr l o)
-        (m <| ObjectMetaV.ResourceVersion' := resource_version |>) 1
+      ObjectMetaV.deepown_l (KObjectV.objectmeta_ptr l o) (m <| ObjectMetaV.ResourceVersion' := resource_version |>) 1
   }}}.
 Proof.
   wp_start as "H". iNamed "H".
   destruct o; simpl in Hi; destruct Hi as [-> _]; wp_method_call;
-    wp_pures; wp_apply (wp_SetResourceVersion_deepown with "[$Hinit $Hmeta]");
+    wp_pures; wp_apply (wp_SetResourceVersion_deepown with "[$Hmeta]");
     iIntros "Hmeta"; iApply "HΦ"; iFrame.
 Qed.
 
 Lemma wp_GetFinalizers_kobject i l o metadata_c dq:
-  {{{ "Hinit" ∷ is_pkg_init code.k8s_io.apimachinery.pkg.apis.meta.v1.pkg_id.v1 ∗
+  {{{ is_pkg_init code.k8s_io.apimachinery.pkg.apis.meta.v1.pkg_id.v1 ∗
       "%Hi" ∷ ⌜ KObjectV.valid_interface i l o ⌝ ∗
       "Hmeta" ∷ (KObjectV.objectmeta_ptr l o) ↦{dq} metadata_c
   }}}
@@ -198,12 +194,12 @@ Lemma wp_GetFinalizers_kobject i l o metadata_c dq:
 Proof.
   wp_start as "H". iNamed "H".
   destruct o; simpl in Hi; destruct Hi as [-> _]; wp_method_call;
-    wp_pures; wp_apply (wp_GetFinalizers with "[$Hinit $Hmeta]");
+    wp_pures; wp_apply (wp_GetFinalizers with "[$Hmeta]");
     iIntros "Hmeta"; iApply "HΦ"; iFrame.
 Qed.
 
 Lemma wp_GetFinalizers_deepown_kobject i l o m dq:
-  {{{ "Hinit" ∷ is_pkg_init code.k8s_io.apimachinery.pkg.apis.meta.v1.pkg_id.v1 ∗
+  {{{ is_pkg_init code.k8s_io.apimachinery.pkg.apis.meta.v1.pkg_id.v1 ∗
       "%Hi" ∷ ⌜ KObjectV.valid_interface i l o ⌝ ∗
       "Hmeta" ∷ ObjectMetaV.deepown_l (KObjectV.objectmeta_ptr l o) m dq
   }}}
@@ -219,30 +215,106 @@ Lemma wp_GetFinalizers_deepown_kobject i l o m dq:
 Proof.
   wp_start as "H". iNamed "H".
   destruct o; simpl in Hi; destruct Hi as [-> _]; wp_method_call;
-    wp_pures; wp_apply (wp_GetFinalizers_deepown with "[$Hinit $Hmeta]");
+    wp_pures; wp_apply (wp_GetFinalizers_deepown with "[$Hmeta]");
     iIntros (sl) "Hfinalizers"; iApply "HΦ"; iFrame.
 Qed.
 
+Lemma wp_GetOwnerReferences_deepown_kobject i l o m dq :
+  {{{ is_pkg_init code.k8s_io.apimachinery.pkg.apis.meta.v1.pkg_id.v1 ∗
+      "%Hi" ∷ ⌜ KObjectV.valid_interface i l o ⌝ ∗
+      "Hmeta" ∷ ObjectMetaV.deepown_l (KObjectV.objectmeta_ptr l o) m dq
+  }}}
+    #(methods i.(interface.ty) "GetOwnerReferences" i.(interface.v)) #()
+  {{{ sl, RET #sl;
+      owner_references_borrow m dq sl (ObjectMetaV.deepown_l (KObjectV.objectmeta_ptr l o) m dq)
+  }}}.
+Proof.
+  wp_start as "H". iNamed "H".
+  destruct o; simpl in Hi; destruct Hi as [-> _]; wp_method_call;
+    wp_pures;
+    wp_apply (wp_GetOwnerReferences_deepown with "[$Hmeta]");
+    iIntros (sl) "Hrefs"; iApply "HΦ"; iExact "Hrefs".
+Qed.
+
+Lemma get_owner_references_capability_kobject i l o dq :
+  KObjectV.valid_interface i l o →
+  ⊢ get_owner_references_capability
+    (interface.ok i) (KObjectV.objectmeta o) dq
+    (KObjectV.deepown_l l o dq).
+Proof.
+  intros Hi. unfold get_owner_references_capability.
+  wp_start as "H". iNamed "H".
+  iPoseProof (KObjectV.deepown_l_split with "Hown") as
+    "(%Hl_nonnull & Htypemeta & Hmeta & Hspec & Hstatus)".
+  wp_pures.
+  iAssert (is_pkg_init code.k8s_io.apimachinery.pkg.apis.meta.v1.pkg_id.v1 ∗
+           ⌜KObjectV.valid_interface i l o⌝ ∗
+           ObjectMetaV.deepown_l (KObjectV.objectmeta_ptr l o) (KObjectV.objectmeta o) dq)%I
+    with "[$Hmeta]" as "Hpre".
+  { iFrame "#". done. }
+  wp_apply (wp_GetOwnerReferences_deepown_kobject i l o with "Hpre").
+  iIntros (sl) "Hrefs".
+  iApply "HΦ".
+  iEval (rewrite /owner_references_borrow) in "Hrefs".
+  iEval (rewrite /owner_references_borrow).
+  iDestruct "Hrefs" as "(%Hnil & Hrefs)".
+  iSplit; first done.
+  destruct (KObjectV.objectmeta o).(ObjectMetaV.OwnerReferences') as
+    [refs|] eqn:Hrefs_some.
+  - iDestruct "Hrefs" as (cs) "(Hsl & Hrefs & Hmeta_restore)".
+    iExists cs. iFrame "Hsl Hrefs".
+    iIntros (cs') "[Hsl Hrefs]".
+    iDestruct ("Hmeta_restore" with "[$Hsl $Hrefs]") as "Hmeta".
+    iApply (KObjectV.deepown_l_restore _ _ _ Hl_nonnull). iFrame.
+  - iApply (KObjectV.deepown_l_restore _ _ _ Hl_nonnull). iFrame.
+Qed.
+
+Lemma wp_GetControllerOf_kobject_exact owner i l o dq :
+  {{{ is_pkg_init code.k8s_io.apimachinery.pkg.apis.meta.v1.pkg_id.v1 ∗
+      "%Howner" ∷ ⌜ owner = interface.ok i ⌝ ∗
+      "%Hi" ∷ ⌜ KObjectV.valid_interface i l o ⌝ ∗
+      "Hobj" ∷ KObjectV.deepown_l l o dq
+  }}}
+    @! code.k8s_io.apimachinery.pkg.apis.meta.v1.v1.GetControllerOf #owner
+  {{{ controller_ref_l, RET #controller_ref_l;
+      KObjectV.deepown_l l o dq ∗
+      (⌜ controller_ref_l = null ∧ meta_parent_ref (KObjectV.objectmeta o) = None ⌝ ∨
+       ∃ controller_ref,
+         ⌜ controller_ref_l ≠ null ∧ is_controller_reference_of (KObjectV.objectmeta o) controller_ref ⌝ ∗
+         OwnerReferenceV.deepown_l controller_ref_l controller_ref 1)
+  }}}.
+Proof.
+  iIntros (Φ) "(#? & H) HΦ". iNamed "H". subst owner.
+  iPoseProof (get_owner_references_capability_kobject i l o dq Hi) as
+    "Hget".
+  iAssert (is_pkg_init code.k8s_io.apimachinery.pkg.apis.meta.v1.pkg_id.v1 ∗
+           get_owner_references_capability (interface.ok i) (KObjectV.objectmeta o) dq
+             (KObjectV.deepown_l l o dq) ∗
+           KObjectV.deepown_l l o dq)%I with "[$Hget $Hobj]" as "Hpre".
+  { iFrame "#". }
+  iApply (wp_GetControllerOf_general_exact with "Hpre").
+  iExact "HΦ".
+Qed.
+
 Lemma wp_SetFinalizers_kobject i l o metadata_c finalizers:
-  {{{ "Hinit" ∷ is_pkg_init code.k8s_io.apimachinery.pkg.apis.meta.v1.pkg_id.v1 ∗
+  {{{ is_pkg_init code.k8s_io.apimachinery.pkg.apis.meta.v1.pkg_id.v1 ∗
       "%Hi" ∷ ⌜ KObjectV.valid_interface i l o ⌝ ∗
       "Hmeta" ∷ (KObjectV.objectmeta_ptr l o) ↦ metadata_c
   }}}
     #(methods i.(interface.ty) "SetFinalizers" i.(interface.v)) #finalizers
   {{{ RET #();
       (KObjectV.objectmeta_ptr l o) ↦
-        (metadata_c <|
-          code.k8s_io.apimachinery.pkg.apis.meta.v1.v1.ObjectMeta.Finalizers' := finalizers |>)
+        (metadata_c <| code.k8s_io.apimachinery.pkg.apis.meta.v1.v1.ObjectMeta.Finalizers' := finalizers |>)
   }}}.
 Proof.
   wp_start as "H". iNamed "H".
   destruct o; simpl in Hi; destruct Hi as [-> _]; wp_method_call;
-    wp_pures; wp_apply (wp_SetFinalizers with "[$Hinit $Hmeta]");
+    wp_pures; wp_apply (wp_SetFinalizers with "[$Hmeta]");
     iIntros "Hmeta"; iApply "HΦ"; iFrame.
 Qed.
 
 Lemma wp_GetDeletionGracePeriodSeconds_kobject i l o metadata_c dq:
-  {{{ "Hinit" ∷ is_pkg_init code.k8s_io.apimachinery.pkg.apis.meta.v1.pkg_id.v1 ∗
+  {{{ is_pkg_init code.k8s_io.apimachinery.pkg.apis.meta.v1.pkg_id.v1 ∗
       "%Hi" ∷ ⌜ KObjectV.valid_interface i l o ⌝ ∗
       "Hmeta" ∷ (KObjectV.objectmeta_ptr l o) ↦{dq} metadata_c
   }}}
@@ -253,30 +325,29 @@ Lemma wp_GetDeletionGracePeriodSeconds_kobject i l o metadata_c dq:
 Proof.
   wp_start as "H". iNamed "H".
   destruct o; simpl in Hi; destruct Hi as [-> _]; wp_method_call;
-    wp_pures; wp_apply (wp_GetDeletionGracePeriodSeconds with "[$Hinit $Hmeta]");
+    wp_pures; wp_apply (wp_GetDeletionGracePeriodSeconds with "[$Hmeta]");
     iIntros "Hmeta"; iApply "HΦ"; iFrame.
 Qed.
 
 Lemma wp_SetDeletionGracePeriodSeconds_kobject i l o metadata_c dgps:
-  {{{ "Hinit" ∷ is_pkg_init code.k8s_io.apimachinery.pkg.apis.meta.v1.pkg_id.v1 ∗
+  {{{ is_pkg_init code.k8s_io.apimachinery.pkg.apis.meta.v1.pkg_id.v1 ∗
       "%Hi" ∷ ⌜ KObjectV.valid_interface i l o ⌝ ∗
       "Hmeta" ∷ (KObjectV.objectmeta_ptr l o) ↦ metadata_c
   }}}
     #(methods i.(interface.ty) "SetDeletionGracePeriodSeconds" i.(interface.v)) #dgps
   {{{ RET #();
       (KObjectV.objectmeta_ptr l o) ↦
-        (metadata_c <|
-          code.k8s_io.apimachinery.pkg.apis.meta.v1.v1.ObjectMeta.DeletionGracePeriodSeconds' := dgps |>)
+        (metadata_c <| code.k8s_io.apimachinery.pkg.apis.meta.v1.v1.ObjectMeta.DeletionGracePeriodSeconds' := dgps |>)
   }}}.
 Proof.
   wp_start as "H". iNamed "H".
   destruct o; simpl in Hi; destruct Hi as [-> _]; wp_method_call;
-    wp_pures; wp_apply (wp_SetDeletionGracePeriodSeconds with "[$Hinit $Hmeta]");
+    wp_pures; wp_apply (wp_SetDeletionGracePeriodSeconds with "[$Hmeta]");
     iIntros "Hmeta"; iApply "HΦ"; iFrame.
 Qed.
 
 Lemma wp_GetDeletionTimestamp_kobject i l o metadata_c dq:
-  {{{ "Hinit" ∷ is_pkg_init code.k8s_io.apimachinery.pkg.apis.meta.v1.pkg_id.v1 ∗
+  {{{ is_pkg_init code.k8s_io.apimachinery.pkg.apis.meta.v1.pkg_id.v1 ∗
       "%Hi" ∷ ⌜ KObjectV.valid_interface i l o ⌝ ∗
       "Hmeta" ∷ (KObjectV.objectmeta_ptr l o) ↦{dq} metadata_c
   }}}
@@ -287,30 +358,29 @@ Lemma wp_GetDeletionTimestamp_kobject i l o metadata_c dq:
 Proof.
   wp_start as "H". iNamed "H".
   destruct o; simpl in Hi; destruct Hi as [-> _]; wp_method_call;
-    wp_pures; wp_apply (wp_GetDeletionTimestamp with "[$Hinit $Hmeta]");
+    wp_pures; wp_apply (wp_GetDeletionTimestamp with "[$Hmeta]");
     iIntros "Hmeta"; iApply "HΦ"; iFrame.
 Qed.
 
 Lemma wp_SetDeletionTimestamp_kobject i l o metadata_c deletion_timestamp:
-  {{{ "Hinit" ∷ is_pkg_init code.k8s_io.apimachinery.pkg.apis.meta.v1.pkg_id.v1 ∗
+  {{{ is_pkg_init code.k8s_io.apimachinery.pkg.apis.meta.v1.pkg_id.v1 ∗
       "%Hi" ∷ ⌜ KObjectV.valid_interface i l o ⌝ ∗
       "Hmeta" ∷ (KObjectV.objectmeta_ptr l o) ↦ metadata_c
   }}}
     #(methods i.(interface.ty) "SetDeletionTimestamp" i.(interface.v)) #deletion_timestamp
   {{{ RET #();
       (KObjectV.objectmeta_ptr l o) ↦
-        (metadata_c <|
-          code.k8s_io.apimachinery.pkg.apis.meta.v1.v1.ObjectMeta.DeletionTimestamp' := deletion_timestamp |>)
+        (metadata_c <| code.k8s_io.apimachinery.pkg.apis.meta.v1.v1.ObjectMeta.DeletionTimestamp' := deletion_timestamp |>)
   }}}.
 Proof.
   wp_start as "H". iNamed "H".
   destruct o; simpl in Hi; destruct Hi as [-> _]; wp_method_call;
-    wp_pures; wp_apply (wp_SetDeletionTimestamp with "[$Hinit $Hmeta]");
+    wp_pures; wp_apply (wp_SetDeletionTimestamp with "[$Hmeta]");
     iIntros "Hmeta"; iApply "HΦ"; iFrame.
 Qed.
 
 Lemma wp_GetGeneration_kobject i l o metadata_c dq:
-  {{{ "Hinit" ∷ is_pkg_init code.k8s_io.apimachinery.pkg.apis.meta.v1.pkg_id.v1 ∗
+  {{{ is_pkg_init code.k8s_io.apimachinery.pkg.apis.meta.v1.pkg_id.v1 ∗
       "%Hi" ∷ ⌜ KObjectV.valid_interface i l o ⌝ ∗
       "Hmeta" ∷ (KObjectV.objectmeta_ptr l o) ↦{dq} metadata_c
   }}}
@@ -321,25 +391,24 @@ Lemma wp_GetGeneration_kobject i l o metadata_c dq:
 Proof.
   wp_start as "H". iNamed "H".
   destruct o; simpl in Hi; destruct Hi as [-> _]; wp_method_call;
-    wp_pures; wp_apply (wp_GetGeneration with "[$Hinit $Hmeta]");
+    wp_pures; wp_apply (wp_GetGeneration with "[$Hmeta]");
     iIntros "Hmeta"; iApply "HΦ"; iFrame.
 Qed.
 
 Lemma wp_SetGeneration_kobject i l o metadata_c generation:
-  {{{ "Hinit" ∷ is_pkg_init code.k8s_io.apimachinery.pkg.apis.meta.v1.pkg_id.v1 ∗
+  {{{ is_pkg_init code.k8s_io.apimachinery.pkg.apis.meta.v1.pkg_id.v1 ∗
       "%Hi" ∷ ⌜ KObjectV.valid_interface i l o ⌝ ∗
       "Hmeta" ∷ (KObjectV.objectmeta_ptr l o) ↦ metadata_c
   }}}
     #(methods i.(interface.ty) "SetGeneration" i.(interface.v)) #generation
   {{{ RET #();
       (KObjectV.objectmeta_ptr l o) ↦
-        (metadata_c <|
-          code.k8s_io.apimachinery.pkg.apis.meta.v1.v1.ObjectMeta.Generation' := generation |>)
+        (metadata_c <| code.k8s_io.apimachinery.pkg.apis.meta.v1.v1.ObjectMeta.Generation' := generation |>)
   }}}.
 Proof.
   wp_start as "H". iNamed "H".
   destruct o; simpl in Hi; destruct Hi as [-> _]; wp_method_call;
-    wp_pures; wp_apply (wp_SetGeneration with "[$Hinit $Hmeta]");
+    wp_pures; wp_apply (wp_SetGeneration with "[$Hmeta]");
     iIntros "Hmeta"; iApply "HΦ"; iFrame.
 Qed.
 
